proof/DenotationSimp.v
@@ -10,6 +10,8 @@ From PLF Require Import WellFormedSimp.
 From Coq Require Import Logic.FunctionalExtensionality.
 From Coq Require Import Logic.ClassicalFacts.
 From Coq Require Import Lists.List.
+From Coq Require Import FunInd.
+From Coq Require Import Recdef.
 
 Import CoreLangSimp.
 Import LinearContext.
@@ -46,6 +48,14 @@ Definition mk_eq_constant c := [[v: constant_basic_type_infer c | (fun _ v => v 
 Definition mk_bot ty := [[v: ty | (fun _ _ => False) ]].
 Definition mk_top ty := [[v: ty | (fun _ _ => True) ]].
 Definition mk_eq_var ty name := [[v: ty | (fun state v => v = (state name)) ]].
+
+Lemma mk_eq_is_well_formed: forall x T phi, well_formed ((x, Oty ({{v:T | phi}}))::nil) (mk_eq_var T x).
+Proof with eauto.
+  intros x T phi. repeat constructor...
+  unfold is_closed_refinement... intros st st'. rewrite t_update_eq. rewrite t_update_eq. reflexivity.
+Qed.
+
+Global Hint Resolve mk_eq_is_well_formed: core.
 
 Lemma mk_eq_constant_spec (c: constant) : empty |- vconst c \in u\_ mk_eq_constant c _/.
 Proof with eauto.
@@ -86,91 +96,241 @@ Definition is_constant (v: value) :=
   end.
 
 (* overtype denotation *)
-Definition over_tmR (ty:overbasety) (c:constant) : Prop :=
-  empty |- c \Vin o\_ ty _/ /\
-            (match ty with
-             | {{v: T | phi }} =>
-                 is_closed_refinement T phi /\ (phi empstate c)
-             end).
+Inductive overbase_tmR: overbasety -> constant -> Prop :=
+| over_tmR_base : forall (T: basic_ty) phi (c: constant),
+    empty |- c \Vin T -> is_closed_refinement T phi -> phi empstate c -> overbase_tmR ({{v: T | phi}}) c.
 
-Inductive is_application: tm -> value -> tm -> Prop :=
-| Is_application: forall (e1: tm) (v2: value) (f x: string),
-    ~ f \FVtm v2 -> is_application e1 v2 (tlete f e1 (tletapp x f v2 x)).
+Lemma over_tmR_has_type: forall T phi c, overbase_tmR ({{v: T | phi}}) c -> empty |- c \Vin T.
+Proof. intros. inversion H. auto. Qed.
 
-(* Inductive under_tmR: underty -> tm -> Prop := *)
-(* | under_tmR_base: forall (T: basic_ty) phi e, *)
+
+Inductive is_application: tm -> tm -> tm -> Prop :=
+| Is_application: forall (e1: tm) (e2: tm) (x1 x2 x3: string),
+    x1 <> x2 -> x2 <> x3 -> x3 <> x1 ->
+    ~ x1 \FVtm e2 ->
+    is_application e1 e2 (tlete x1 e1
+                                (tlete x2 e2
+                                       (tletapp x3 x1 x2 x3)
+                                )
+                         ).
+
+Global Hint Constructors is_application: core.
+
+(* Inductive underbase_tmR: underty -> tm -> Prop := *)
+(* | under_tmR_base : forall (T: basic_ty) phi (e: tm), *)
 (*     empty |- e \in T -> is_closed_refinement T phi -> *)
-(*                   (forall (c: constant), empty |- vconst c \Vin T -> *)
-(*                                             (phi empstate c -> e -->* (vconst c))) -> *)
-(*                   under_tmR ([[v: T | phi]]) e *)
-(* | under_tmR_oarr: forall x t1 t2 e, *)
+(*                   (forall (c: constant), *)
+(*                       empty |- vconst c \Vin T -> *)
+(*                               phi empstate c -> *)
+(*                               e -->* (vconst c) *)
+(*                   ) -> underbase_tmR ([[v: T | phi]]) e. *)
+
+(* Inductive under_fo_tmR: underty -> tm -> Prop := *)
+(* | under_fo_tmR_base : forall (T: basic_ty) phi (e: tm), *)
+(*     empty |- e \in T -> is_closed_refinement T phi -> *)
+(*                   (forall (c: constant), *)
+(*                       empty |- vconst c \Vin T -> *)
+(*                               phi empstate c -> *)
+(*                               e -->* (vconst c) *)
+(*                   ) -> under_fo_tmR ([[v: T | phi]]) e *)
+(* | under_fo_tmR_oarr: forall (x: string) (t1: overbasety) (t2: underty) (e: tm), *)
 (*     empty |- e \in u\_ x o: t1 o--> t2 _/ -> *)
 (*                            (forall (c_x: constant), *)
-(*                                over_tmR t1 c_x -> *)
-(*                                (forall e3, is_application e c_x e3 -> under_tmR (under_subst_c x c_x t2) e3)) -> *)
-(*                            under_tmR (x o: t1 o--> t2) e *)
-(* | under_tmR_arrarr: forall t1 t2 e, *)
+(*                                overbase_tmR t1 c_x -> *)
+(*                                (forall e3, is_application e c_x e3 -> under_fo_tmR (under_subst_c x c_x t2) e3) *)
+(*                            ) -> under_fo_tmR (x o: t1 o--> t2) e. *)
+
+(* Lemma under_fo_tmR_has_type: forall tau c, under_fo_tmR tau c -> empty |- c \in u\_ tau _/. *)
+(* Proof. intros. inversion H; auto. Qed. *)
+
+
+Fixpoint num_arr_sym_arr (tau: underarrowty): nat :=
+  match tau with
+  | x o: t1 o--> t2 => 1 + (num_arr_sym t2)
+  | t1 u--> t2 => (num_arr_sym_arr t1) + (num_arr_sym t2)
+  end
+with num_arr_sym (tau: underty): nat :=
+       match tau with
+       | [[v: _ | _ ]] => 0
+       | ArrowUnder tau => num_arr_sym_arr tau
+       end.
+
+Definition num_arr_sym_order (t1 t2: underty) :=
+  num_arr_sym t1 < num_arr_sym t2.
+
+Global Hint Constructors Acc: core.
+
+Lemma num_arr_sym_order_wf' : forall num, forall tau, num_arr_sym tau <= num -> Acc num_arr_sym_order tau.
+Admitted.
+
+Theorem num_arr_sym_order_wf : well_founded num_arr_sym_order.
+  red; intro; eapply num_arr_sym_order_wf'; eauto.
+Defined.
+
+Lemma under_subst_c_wf: forall x c_x t2, num_arr_sym_order (under_subst_c x c_x t2) t2.
+Admitted.
+
+Global Hint Resolve under_subst_c_wf: core.
+
+
+(* Cannot figure out mutual recursive definition. *)
+Lemma underty_wf_arrarr_arr1: forall (t1:underarrowty) (t2: underty), num_arr_sym_order t1 t2.
+Admitted.
+
+Lemma underty_wf_arrarr_arr2: forall (t1:underty) (t2: underty), num_arr_sym_order t1 t2.
+Admitted.
+
+Lemma underty_wf_subst: forall (t1:underty) (t2: underty), num_arr_sym_order t1 t2.
+Admitted.
+
+Definition under_tmR_wf: underty -> tm -> Prop.
+Proof.
+  refine (@well_founded_induction_type
+            underty num_arr_sym_order
+            num_arr_sym_order_wf
+            (fun _ => tm -> Prop)
+            (fun (ty: underty)
+               (under_tmR_wf: forall (tau': underty), num_arr_sym_order tau' ty -> tm -> Prop)
+               (e: tm) =>
+               empty |- e \in u\_ ty _/ /\
+                               (match ty with
+                                | [[v: T | phi ]] =>
+                                    is_closed_refinement T phi /\
+                                      (forall (c: constant),
+                                          empty |- vconst c \Vin T ->
+                                                  (phi empstate c -> e -->* (vconst c))
+                                      )
+                                | x o: t1 o--> t2 =>
+                                    forall (c_x: constant),
+                                      overbase_tmR t1 c_x ->
+                                      (forall e3, is_application e c_x e3 ->
+                                             under_tmR_wf (under_subst_c x c_x t2)
+                                                           (underty_wf_subst (under_subst_c x c_x t2) ty) e3)
+                                | t1 u--> t2 =>
+                                    forall (e_x: tm),
+                                      under_tmR_wf t1 (underty_wf_arrarr_arr1 t1 ty) e_x ->
+                                      (forall e3, is_application e e_x e3 -> under_tmR_wf t2 (underty_wf_arrarr_arr2 t2 ty) e3)
+                                end)
+            )
+         ).
+Qed.
+
+Definition under_tmR_spec_base: forall (T: basic_ty) phi (e: tm),
+    under_tmR_wf ([[v: T | phi]]) e <->
+    empty |- e \in T /\ is_closed_refinement T phi /\
+                    (forall (c: constant),
+                        empty |- vconst c \Vin T ->
+                                phi empstate c ->
+                                e -->* (vconst c)
+                    ).
+Admitted.
+
+Definition under_tmR_spec_arrarr: forall (t1: underarrowty) (t2: underty) (e: tm),
+    under_tmR_wf (t1 u--> t2) e <->
+    empty |- e \in u\_ t1 u--> t2 _/ /\
+                    (forall (v_x: value),
+                        under_tmR_wf t1 v_x ->
+                        (forall e3, is_application e v_x e3 -> under_tmR_wf t2 e3)
+                    ).
+Admitted.
+
+Definition under_tmR_spec_oarr: forall (x: string) (t1: overbasety) (t2: underty) (e: tm),
+    under_tmR_wf (x o: t1 o--> t2) e <->
+    empty |- e \in u\_ x o: t1 o--> t2 _/ /\
+                             (forall (c_x: constant),
+                                 overbase_tmR t1 c_x ->
+                                 (forall e3, is_application e c_x e3 -> under_tmR_wf (under_subst_c x c_x t2) e3)
+                             ).
+Admitted.
+
+(* Non strictly positive occurrence  *)
+(* Inductive under_tmR: underty -> tm -> Prop := *)
+(* | under_tmR_base : forall (T: basic_ty) phi (e: tm), *)
+(*     empty |- e \in T -> is_closed_refinement T phi -> *)
+(*                   (forall (c: constant), *)
+(*                       empty |- vconst c \Vin T -> *)
+(*                               phi empstate c -> *)
+(*                               e -->* (vconst c) *)
+(*                   ) -> under_tmR ([[v: T | phi]]) e *)
+(* | under_tmR_arrarr: forall (t1 t2: underarrowty) (e: tm), *)
 (*     empty |- e \in u\_ t1 u--> t2 _/ -> *)
-(*                   ( forall (e_x: tm), *)
-(*                       under_tmR t1 e_x -> *)
-(*                       (forall (v_x: value), *)
-(*                           empty |- v_x \Vin u\_ t1 _/ -> *)
-(*                                   e -->* v_x -> *)
-(*                                   (forall e3, is_application e v_x e3 -> under_tmR t2 e3) *)
-(*                   )) -> *)
-(*                   under_tmR (t1 u--> t2) e. *)
+(*                   (forall (v_x: value), *)
+(*                       under_tmR t1 v_x -> *)
+(*                       (forall e3, is_application e v_x e3 -> under_tmR t2 e3) *)
+(*                   ) -> under_tmR (t1 u--> t2) e. *)
+(* | under_tmR_oarr: forall (x: string) (t1: overbasety) (t2: underty) (e: tm), *)
+(*     empty |- e \in u\_ x o: t1 o--> t2 _/ -> *)
+(*                            (forall (c_x: constant), *)
+(*                                overbase_tmR t1 c_x -> *)
+(*                                (forall e3, is_application e c_x e3 -> under_tmR_aux (under_subst_c x c_x t2) e3) *)
+(*                            ) -> under_tmR (t1 u--> t2) e. *)
 
+(* A wrong imp *)
+(* Fixpoint under_arr_tmR_aux (ty:underarrowty) (e:tm) : Prop := *)
+(*   empty |- e \in u\_ ty _/ /\ *)
+(*                   (match ty with *)
+(*                    | x o: t1 o--> t2 => False *)
+(*                    | t1 u--> t2 => *)
+(*                        forall (e_x: tm), *)
+(*                          under_arr_tmR_aux t1 e_x -> *)
+(*                          (forall e3, is_application e e_x e3 -> under_tmR_aux t2 e3) *)
+(*                    end) *)
+(* with under_tmR_aux (ty:underty) (e:tm) : Prop := *)
+(*        (match ty with *)
+(*         | [[v: T | phi ]] => *)
+(*             empty |- e \in u\_ ty _/ /\ *)
+(*                             is_closed_refinement T phi /\ *)
+(*                             (forall (c: constant), *)
+(*                                 empty |- vconst c \Vin T -> *)
+(*                                         (phi empstate c -> e -->* (vconst c)) *)
+(*                             ) *)
+(*         | ArrowUnder ty => under_arr_tmR_aux ty e *)
+(*         end). *)
 
-Fixpoint under_arr_tmR_aux (ty:underarrowty) (e:tm) : Prop :=
-  empty |- e \in u\_ ty _/ /\
-                  (match ty with
-                   | x o: t1 o--> t2 => False
-                   | t1 u--> t2 =>
-                       forall (e_x: tm),
-                         under_arr_tmR_aux t1 e_x ->
-                         (forall (v_x: value),
-                             empty |- v_x \Vin u\_ t1 _/ ->
-                                     e -->* v_x ->
-                                     (forall e3, is_application e v_x e3 -> under_tmR_aux t2 e3)
-                         )
-                   end)
-with under_tmR_aux (ty:underty) (e:tm) : Prop :=
-       empty |- e \in u\_ ty _/ /\
-                       (match ty with
-                        | [[v: T | phi ]] =>
-                            is_closed_refinement T phi /\
-                              (forall (c: constant),
-                                  empty |- vconst c \Vin T ->
-                                          (phi empstate c -> e -->* (vconst c))
-                              )
-                        | ArrowUnder ty => under_arr_tmR_aux ty e
-                        end).
+(* Definition under_tmR (ty:underty) (e:tm) : Prop := *)
+(*   (match ty with *)
+(*    | [[v: _ | _ ]] => under_tmR_aux ty e *)
+(*    | _ u--> _ => under_tmR_aux ty e *)
+(*    | x o: t1 o--> t2 => *)
+(*        empty |- e \in u\_ ty _/ /\ *)
+(*                        forall (c_x: constant), *)
+(*                          overbase_tmR t1 c_x -> (forall e3, is_application e c_x e3 -> under_tmR_aux (under_subst_c x c_x t2) e3) *)
+(*    end). *)
 
-Definition under_tmR (ty:underty) (e:tm) : Prop :=
-  empty |- e \in u\_ ty _/ /\
-                  (match ty with
-                   | [[v: _ | _ ]] => under_tmR_aux ty e
-                   | _ u--> _ => under_tmR_aux ty e
-                   | x o: t1 o--> t2 =>
-                       forall (c_x: constant),
-                         over_tmR t1 c_x -> (forall e3, is_application e c_x e3 -> under_tmR_aux (under_subst_c x c_x t2) e3)
-                   end).
+Definition under_tmR := under_tmR_wf.
+
+Lemma under_tmR_has_type: forall tau e, under_tmR tau e -> empty |- e \in u\_ tau _/.
+Proof with eauto.
+  intros.
+  destruct tau.
+  - rewrite under_tmR_spec_base in H. destruct H...
+  - destruct u.
+    + rewrite under_tmR_spec_oarr in H. destruct H...
+    + rewrite under_tmR_spec_arrarr in H. destruct H...
+Qed.
+
+Global Hint Resolve under_tmR_has_type: core.
 
 Inductive tmR: overunderty -> tm -> Prop :=
-| tmR_oty: forall oty c, over_tmR oty c -> tmR oty c
+| tmR_oty: forall oty c, overbase_tmR oty c -> tmR oty c
 | tmR_uty: forall uty e, under_tmR uty e -> tmR uty e.
+
+Lemma denotation_has_basic_type: forall tau e, tmR tau e -> empty |- e \in ou\_ tau _/.
+Admitted.
+
+Global Hint Constructors tmR: core.
 
 Lemma tmR_constant (c: constant): tmR (mk_eq_constant c) (vconst c).
 Proof with eauto.
-  constructor. split; auto.
-  destruct c; simpl; split; auto; split; intros; subst...
+  constructor.
+  destruct c; simpl; unfold mk_eq_constant; rewrite under_tmR_spec_base; split; auto; split; intros; subst...
 Qed.
 
 Global Hint Resolve tmR_constant: core.
 
-Fixpoint ty_subst_under_ctx (id:string) (c_id: constant) (Gamma: context) (tau: underty) : context * underty :=
+Fixpoint ty_subst_under_ctx (id:string) (c_id: constant) (Gamma: context) (tau: overunderty) : context * overunderty :=
   match Gamma with
-  | nil => (Gamma, underty_subst id c_id tau)
+  | nil => (Gamma, overunderty_subst id c_id tau)
   | (x, xty) :: Gamma =>
       if String.eqb x id
       then
@@ -180,51 +340,71 @@ Fixpoint ty_subst_under_ctx (id:string) (c_id: constant) (Gamma: context) (tau: 
         ((x, overunder_subst_c id c_id xty) :: Gamma', tau')
   end.
 
-Lemma ty_subst_under_ctx_not_in_ctx (id:string) (c_id: constant) (Gamma: context) (tau: underty):
+(* Definition ty_subst_under_ctx_prop (id:string) (c_id: constant) (Gamma: context) (tau: overunderty) (Gamma': context) (tau': overunderty) := ty_subst_under_ctx id c_id Gamma tau = (Gamma', tau'). *)
+
+Lemma ty_subst_under_ctx_not_in_ctx (id:string) (c_id: constant) (Gamma: context) (tau: overunderty):
   l_find_right_most Gamma id = None ->
-  ty_subst_under_ctx id c_id Gamma tau = (Gamma, (underty_subst id c_id tau)).
+  ty_subst_under_ctx id c_id Gamma tau = (Gamma, (overunderty_subst id c_id tau)).
 Admitted.
 
+Fixpoint name_not_free_in_ctx_and_ty (id:string) (Gamma: context) (tau: overunderty):=
+  match Gamma with
+  | nil => ~ id \FVty tau
+  | (x, xty)::Gamma =>
+      ~ id \FVty xty /\
+        if String.eqb x id then True else name_not_free_in_ctx_and_ty id Gamma tau
+  end.
 
-Inductive tmR_in_ctx: context -> underty -> tm -> Prop :=
-| tmR_in_ctx_nil: forall (ty: underty) e, tmR ty e -> tmR_in_ctx [] ty e
-| tmR_in_ctx_cons_over: forall (x: string) (T:basic_ty) (phi: refinement) (Gamma: context) tau e,
-    (forall c_x Gamma' tau', over_tmR ({{v: T | phi}}) c_x ->
-                        (Gamma', tau') = ty_subst_under_ctx x c_x Gamma tau ->
-                        tmR_in_ctx Gamma' tau' (subst x (vconst c_x) e)) ->
-    tmR_in_ctx ((x, (Oty ({{v: T | phi}}))) :: Gamma) tau e
-| tmR_in_ctx_cons_under: forall (x: string) (T:basic_ty) (phi: refinement) (Gamma: context) tau e,
-    (exists e_x, under_tmR ([[v: T | phi]]) e_x /\
-              (forall (c_x: constant) Gamma' tau',
-                  empty |- (vconst c_x) \Vin T -> e_x -->* (vconst c_x) ->
-                          (Gamma', tau') = ty_subst_under_ctx x c_x Gamma tau ->
-                          tmR_in_ctx Gamma' tau' (subst x (vconst c_x) e))) ->
+Inductive tmR_in_ctx: context -> overunderty -> tm -> Prop :=
+| tmR_in_ctx_nil: forall (ty: overunderty) e, tmR ty e -> tmR_in_ctx [] ty e
+| tmR_in_ctx_cons_overbase: forall (x: string) (tau_x: overbasety) (Gamma: context) (tau: overunderty) e,
+    (forall c_x Gamma' (tau': overunderty),
+        overbase_tmR tau_x c_x ->
+        ty_subst_under_ctx x c_x Gamma tau = (Gamma', tau') ->
+        tmR_in_ctx Gamma' tau' (tlete x (vconst c_x) e)) ->
+    tmR_in_ctx ((x, (Oty tau_x)) :: Gamma) tau e
+| tmR_in_ctx_cons_underbase: forall (x: string) (T:basic_ty) (phi: refinement) (Gamma: context) (tau: overunderty) e,
+    (exists e_x_hat, under_tmR ([[v: T | phi]]) e_x_hat /\
+                  (forall e_x, under_tmR ([[v: T | phi]]) e_x ->
+                          (forall (c_x: constant) Gamma' (tau': overunderty),
+                              empty |- (vconst c_x) \Vin T -> e_x_hat -->* (vconst c_x) ->
+                                      ty_subst_under_ctx x c_x Gamma tau = (Gamma', tau') ->
+                                      tmR_in_ctx Gamma' tau' (tlete x e_x e))
+                  )
+    ) ->
     tmR_in_ctx ((x, (Uty ([[v: T | phi]]))) :: Gamma) tau e
-| tmR_in_ctx_cons_ind_arrow: forall (x: string) t1 t2 (Gamma: context) (ty: underty) e,
-    (exists e_x, under_tmR (t1 u--> t2) e_x /\
-              tmR_in_ctx Gamma ty (tlete x e_x e)) ->
-    tmR_in_ctx ((x, Uty (t1 u--> t2)) :: Gamma) ty e
-| tmR_in_ctx_cons_d_arrow: forall (x: string) (y: string) (t1: overbasety) (t2: underty) (Gamma: context) (ty: underty) e,
-    (exists e_x, under_tmR (y o: t1 o--> t2) e_x /\
-              tmR_in_ctx Gamma ty (tlete x e_x e)) ->
-    tmR_in_ctx ((x, Uty (y o: t1 o--> t2)) :: Gamma) ty e.
+| tmR_in_ctx_cons_underarr: forall (x: string) (tau_x: underarrowty) (Gamma: context) (tau: overunderty) e,
+    (forall e_x, under_tmR tau_x e_x ->
+            tmR_in_ctx Gamma tau (tlete x e_x e)) ->
+    tmR_in_ctx ((x, Uty tau_x) :: Gamma) tau e.
 
 Global Hint Constructors tmR_in_ctx: core.
 
-Lemma tmR_in_ctx_pre_weakening: forall Gamma1 Gamma2 Gamma3 (tau: underty),
-    (Gamma1 ++ Gamma2) = Gamma3 ->
-    well_formed Gamma2 tau ->
-    (forall e, tmR_in_ctx Gamma2 tau e -> tmR_in_ctx Gamma3 tau e).
+
+Lemma tmR_in_ctx_preserve_oarr: forall Gamma x (tau_x: overbasety) e (tau: underty),
+    tmR_in_ctx (Gamma <l> x :l: Oty tau_x) tau e ->
+    tmR_in_ctx Gamma (x o: tau_x o--> tau) (vlam x (o\_ tau_x _/) e).
 Admitted.
 
-Definition context_not_free_in_term {A: Type} (ctx: linear_context A) (e: tm): Prop.
+Lemma tmR_in_ctx_preserve_arrarr: forall Gamma x (tau_x: underarrowty) e (tau: underty),
+    tmR_in_ctx (Gamma <l> x :l: Uty tau_x) tau e ->
+    tmR_in_ctx Gamma (tau_x u--> tau) (vlam x (u\_ tau_x _/) e).
 Admitted.
 
-Definition context_not_free_in_underty {A: Type} (ctx: linear_context A) (tau: underty): Prop.
+Lemma tmR_in_ctx_preserve_arrarr_application: forall Gamma x (v1 v2: value) tau tau1,
+    tmR_in_ctx Gamma (tau1 u--> tau) v1 ->
+    tmR_in_ctx Gamma tau1 v2 ->
+    tmR_in_ctx Gamma tau (tletapp x v1 v2 x).
 Admitted.
 
-Lemma tmR_in_ctx_post_weakening: forall Gamma (tau: underty),
-    well_formed l_empty tau ->
-    (forall e, tmR_in_ctx l_empty tau e -> tmR_in_ctx Gamma tau e).
-Proof with eauto.
+Lemma tmR_in_ctx_preserve_oarr_c_application: forall Gamma x (v1: value) (c2: constant) tau a T phi,
+    tmR_in_ctx Gamma (a o: {{v: T | phi}} o--> tau) v1 ->
+    tmR_in_ctx Gamma ([[v: T | phi]]) c2 ->
+    tmR_in_ctx Gamma (under_subst_c a c2 tau) (tletapp x v1 c2 x).
+Admitted.
+
+Lemma tmR_in_ctx_preserve_oarr_var_application: forall Gamma x (v1: value) (name2: string) tau a T phi,
+    tmR_in_ctx Gamma (a o: {{v: T | phi}} o--> tau) v1 ->
+    tmR_in_ctx Gamma ([[v: T | phi]]) name2 ->
+    tmR_in_ctx Gamma (under_subst_id a name2 tau) (tletapp x v1 name2 x).
 Admitted.
