proof/TypingRules.v
@@ -6,6 +6,8 @@ From PLF Require Import LinearContext.
 From PLF Require Import RfTypeDef.
 From PLF Require Import WellFormedSimp.
 From PLF Require Import DenotationSimp.
+From PLF Require Import CtxInvariantSimp.
+From PLF Require Import TypeDisj.
 From PLF Require Import SubtypingSimp.
 From Coq Require Import Logic.FunctionalExtensionality.
 From Coq Require Import Logic.ClassicalFacts.
@@ -15,16 +17,21 @@ Import CoreLangSimp.
 Import LinearContext.
 Import WellFormedSimp.
 Import DenotationSimp.
+Import CtxInvariantSimp.
+Import TypeDisj.
 Import SubtypingSimp.
 Import ListNotations.
 
-Definition apply_op_over_refinements op (phi1 phi2: refinement): refinement :=
-  (fun st v =>
-     forall n1 n2, phi1 st (cnat n1) -> phi2 st (cnat n2) ->
-              v = (apply_op op n1 n2)).
+(* Definition apply_op_over_refinements op (phi1 phi2: refinement): refinement := *)
+(*   (fun st v => *)
+(*      forall n1 n2, phi1 st (cnat n1) -> phi2 st (cnat n2) -> *)
+(*               v = (apply_op op n1 n2)). *)
 
-Definition mk_op_retty op (phi1 phi2: refinement) :=
-  (BaseUnder (op_ret_ty op) (apply_op_over_refinements op phi1 phi2)).
+(* Definition mk_op_retty op (phi1 phi2: refinement) := *)
+(*   (BaseUnder (op_ret_ty op) (apply_op_over_refinements op phi1 phi2)). *)
+
+(* Definition apply_op_from_cids (op: biop) (cid1 cid2: cid): tm := *)
+(* (apply_op op n1 n2). *)
 
 Definition const_order: constant -> constant -> Prop.
 Admitted.
@@ -36,70 +43,48 @@ Reserved Notation "Gamma '\C-' t '\Tin' T" (at level 40).
 Reserved Notation "Gamma '\C-' t '\Vin' T" (at level 40).
 
 Inductive term_under_type_chek : context -> tm -> underty -> Prop :=
-| UT_Value: forall Gamma v uty,
-    well_formed_ctx Gamma ->
-    Gamma \C- v \Vin uty -> Gamma \C- (tvalue v) \Tin uty
-| UT_Exn: forall Gamma T,
-    well_formed_ctx Gamma ->
-    Gamma \C- texn \Tin (mk_bot T)
+| UT_Value: forall Gamma v uty, Gamma \C- v \Vin uty -> Gamma \C- (tvalue v) \Tin uty
+| UT_Exn: forall Gamma T, ctx_inv Gamma -> Gamma \C- texn \Tin (mk_bot T)
 | UT_Sub: forall Gamma e tau1 tau2,
-    l_empty \C- e \Tin tau1 ->
-    l_empty  \C- tau1 \<: tau2 ->
-    well_formed l_empty tau2 ->
-    well_formed_ctx Gamma ->
+    l_empty \C- e \Tin tau1 -> l_empty  \C- tau1 \<: tau2 ->
+    well_formed l_empty tau2 -> ctx_inv Gamma ->
+    Gamma \C- e \Tin tau2
+| UT_Eq: forall Gamma e tau1 tau2,
+    Gamma \C- e \Tin tau1 ->
+    Gamma \C- tau1 \<: tau2 -> Gamma \C- tau2 \<: tau1 ->
+    well_formed Gamma tau2 -> ctx_inv Gamma ->
     Gamma \C- e \Tin tau2
 | UT_Merge: forall Gamma e (tau1 tau2 tau3: underty),
-    Gamma \C- e \Tin tau1 ->
-    Gamma \C- e \Tin tau2 ->
-    (Gamma \C- tau1 \tyor tau2 \tyeq tau3) ->
+    Gamma \C- e \Tin tau1 -> Gamma \C- e \Tin tau2 -> (Gamma \C- tau1 \tyor tau2 \tyeq tau3) ->
     well_formed l_empty tau3 ->
     Gamma \C- e \Tin tau3
-| UT_Lete: forall (Gamma: context) x e_x tau_x tau_x' e tau,
-    Gamma \C- e_x \Tin tau_x ->
-    Gamma \C- tau_x \<: tau_x' ->
-    (Gamma <l> x :l: tau_x') \C- e \Tin tau ->
-    Gamma \< ((x, Uty tau_x')::nil) \> \C- tau ->
+| UT_Lete: forall (Gamma: context) x e_x e tau, forall tau_x,
+    Gamma \C- e_x \Tin tau_x -> (Gamma <l> x :l: tau_x) \C- e \Tin tau ->
+    well_formed Gamma tau ->
     Gamma \C- (tlete x e_x e) \Tin tau
-| UT_LetOp: forall (Gamma: context) x op v1 v2 phi1 phi2 tau_x' e tau,
+| UT_LetOp: forall (Gamma: context) x op (v1 v2: cid) e tau, forall phi1 phi2,
     Gamma \C- v1 \Vin [[v: TNat | phi1 ]] ->
     Gamma \C- v2 \Vin [[v: TNat | phi2 ]] ->
-    Gamma \C- (mk_op_retty op phi1 phi2) \<: tau_x' ->
-    (Gamma <l> x :l: tau_x') \C- e \Tin tau ->
-    Gamma \< ((x, Uty tau_x')::nil) \> \C- tau ->
+    (Gamma <l> x :l: (mk_op_retty_from_cids op v1 v2)) \C- e \Tin tau ->
+    well_formed Gamma tau ->
     Gamma \C- (tletbiop x op v1 v2 e) \Tin tau
-| UT_LetAppIndepend: forall Gamma x v1 v2 e tauarg tau_x tau_x' tau,
-    Gamma \C- v1 \Vin (tauarg u--> tau_x) ->
-    Gamma \C- v2 \Vin tauarg ->
-    Gamma \C- tau_x \<: tau_x' ->
-    (Gamma <l> x :l: tau_x') \C- e \Tin tau ->
-    Gamma \< ((x, Uty tau_x')::nil) \> \C- tau ->
+| UT_LetAppIndepend: forall Gamma x v1 v2 e tau, forall tauarg tau_x,
+    Gamma \C- v1 \Vin (tauarg u--> tau_x) -> Gamma \C- v2 \Vin tauarg ->
+    (Gamma <l> x :l: tau_x) \C- e \Tin tau ->
+    well_formed Gamma tau ->
     Gamma \C- (tletapp x v1 v2 e) \Tin tau
 (* the value can only be constant or variables *)
-| UT_LetAppDepend1: forall Gamma x v1 (c2: constant) e T phi a tau_x tau_x' tau,
-    Gamma \C- v1 \Vin (a o: {{v: T | phi}} o--> tau_x) ->
-    Gamma \C- c2 \Vin [[v: T | phi]] ->
-    Gamma \C- (under_subst_c a c2 tau_x) \<: tau_x' ->
-    (Gamma <l> x :l: tau_x') \C- e \Tin tau ->
-    Gamma \< ((x, Uty tau_x')::nil) \> \C- tau ->
+| UT_LetAppDepend1: forall Gamma x v1 (c2: cid) e tau, forall T phi a tau_x,
+    Gamma \C- v1 \Vin (a o: {{v: T | phi}} o--> tau_x) -> Gamma \C- c2 \Vin [[v: T | phi]] ->
+   (Gamma <l> x :l:(under_subst_cid a c2 tau_x)) \C- e \Tin tau ->
+    well_formed Gamma tau ->
     Gamma \C- (tletapp x v1 c2 e) \Tin tau
-| UT_LetAppDepend2: forall Gamma x v1 (x2: string) e T phi a tau_x tau_x' tau,
-    Gamma \C- v1 \Vin (a o: {{v: T | phi}} o--> tau_x) ->
-    Gamma \C- x2 \Vin [[v: T | phi]] ->
-    Gamma \C- (under_subst_id a x2 tau_x) \<: tau_x' ->
-    (Gamma <l> x :l: tau_x') \C- e \Tin tau ->
-    Gamma \< ((x, Uty tau_x')::nil) \> \C- tau ->
-    Gamma \C- (tletapp x v1 x2 e) \Tin tau
 with value_under_type_check : context -> value -> underty -> Prop :=
-| UT_Contant: forall Gamma c,
-    well_formed_ctx Gamma ->
-    Gamma \C- (vconst c) \Vin (mk_eq_constant c)
+| UT_Contant: forall Gamma c, ctx_inv Gamma -> Gamma \C- (vconst c) \Vin (mk_eq_constant c)
 | UT_VarUnder: forall Gamma x (tau: underty),
-    well_formed_ctx Gamma ->
-    l_find_right_most Gamma x = Some (Uty tau) ->
-    Gamma \C- (vvar x) \Vin tau
+    ctx_inv Gamma -> l_find_right_most Gamma x = Some (Uty tau) ->  Gamma \C- (vvar x) \Vin tau
 | UT_VarOver: forall Gamma T x,
-    well_formed_ctx Gamma ->
-    (exists phi, l_find_right_most Gamma x = Some (Oty ({{v: T | phi}}))) ->
+    ctx_inv Gamma -> (exists phi, l_find_right_most Gamma x = Some (Oty ({{v: T | phi}}))) ->
     Gamma \C- (vvar x) \Vin (mk_eq_var T x)
 | UT_LamDep: forall Gamma x tau_x e tau,
     well_formed Gamma (x o: tau_x o--> tau) ->
@@ -115,6 +100,17 @@ where
 Scheme value_under_type_check_rec := Induction for value_under_type_check Sort Prop
     with term_under_type_chek_rec := Induction for term_under_type_chek Sort Prop.
 
-Lemma type_judgement_implies_well_formed: forall Gamma e tau,
-    Gamma \C- e \Tin tau -> well_formed_ctx Gamma /\ well_formed Gamma tau.
+(* Definition mk_op_retty_spec: forall Gamma op (cid1 cid2: cid) (phi1 phi2: refinement), *)
+(*     ctx_inv Gamma -> *)
+(*     Gamma \C- cid1 \Vin [[v:TNat | phi1]] -> *)
+(*     Gamma \C- cid2 \Vin [[v:TNat | phi2]] -> *)
+(*     tmR_in_ctx Gamma (mk_op_retty_from_cids op cid1 cid2) (apply_op op n1 n2). *)
+(* Admitted. *)
+
+Lemma type_judgement_implies_inv: forall Gamma e tau,
+    Gamma \C- e \Tin tau -> ctx_inv Gamma /\ well_formed Gamma tau.
+Admitted.
+
+Lemma type_judgement_implies_basic_type_judgement: forall Gamma e tau,
+    Gamma \C- e \Tin tau -> (lctx_to_basic_ctx Gamma) |- e \in u\_ tau _/.
 Admitted.
