proof/ClosingOperationSimp.v
@@ -1,0 +1,80 @@
+Set Warnings "-notation-overridden,-parsing".
+From PLF Require Import Maps.
+From PLF Require Import CoreLangSimp.
+From PLF Require Import NormalTypeSystemSimp.
+From PLF Require Import LinearContext.
+From PLF Require Import RfTypeDef.
+From PLF Require Import WellFormedSimp.
+From PLF Require Import DenotationSimp.
+From PLF Require Import CtxInvariantSimp.
+From Coq Require Import Logic.FunctionalExtensionality.
+From Coq Require Import Logic.ClassicalFacts.
+From Coq Require Import Lists.List.
+
+Import CoreLangSimp.
+Import LinearContext.
+Import WellFormedSimp.
+Import DenotationSimp.
+Import CtxInvariantSimp.
+Import ListNotations.
+
+Definition close_phi_to (x: string) (T: basic_ty) (phi: refinement) (tau: overunderty): overunderty.
+Admitted.
+
+Definition close_underty_to (x: string) (tau_x: underty) (tau: overunderty) :=
+  match tau_x with
+  | [[v: T | phi ]] => close_phi_to x T phi tau
+  | _ => tau
+  end.
+
+Lemma close_underty_to_spec: forall Gamma (x: string) (tau_x: underty) (tau: overunderty),
+    ctx_inv (Gamma ++ ((x, Uty tau_x)::nil)) ->
+    (forall e, tmR_in_ctx (Gamma ++ ((x, Uty tau_x)::nil)) tau e <->
+            tmR_in_ctx (Gamma ++ ((x, Uty tau_x)::nil)) (close_underty_to x tau_x tau) e).
+Admitted.
+
+Lemma ty_subst_under_empty_ctx_not_free: forall x c_x tau,
+    ~ appear_free_in_underty x tau ->
+    ty_subst_under_ctx x c_x nil tau = (nil, Uty tau).
+Admitted.
+
+Lemma denotation_spec: forall (tau tau_x: underty) x e,
+    ~ appear_free_in_underty x tau ->
+    tmR_in_ctx [(x, Uty tau_x)] tau e ->
+    (forall e_x, under_tmR tau_x e_x -> (exists v : value, e_x -->* v)) ->
+    (forall e_x,
+        under_tmR tau_x e_x ->
+        under_tmR tau (tlete x e_x e)
+    ).
+Proof with eauto.
+  intros tau tau_x x e Hfree HeD Hnoterr e_x HexD.
+  inversion HeD; simpl; subst.
+  - destruct H4 as (e_x_hat & HexhatD & HH).
+    assert (empty |- e_x_hat \in T)... apply under_tmR_has_type in HexhatD...
+    apply Hnoterr in HexhatD.
+    destruct HexhatD as (v_x_hat & HEv_x_hat).
+    assert (empty |- v_x_hat \Vin T) as HTc_x_hat. apply preservation_value with (t:=e_x_hat)...
+    assert (exists (c_x_hat: constant), v_x_hat = c_x_hat). apply basic_value_const_exists in HTc_x_hat... destruct H0 as (c_x_hat & H0)...
+    subst.
+    eapply HH with (Gamma':=nil) (tau':=tau) in HexD...
+    + inversion HexD; subst. inversion H0; subst...
+    + apply ty_subst_under_empty_ctx_not_free...
+  - apply H4 in HexD. inversion HexD; subst. inversion H; subst...
+Qed.
+
+Lemma ctx_inv_implies_drop_right_most: forall Gamma (x: string) (tau_x: underty) (tau: underty),
+    ctx_inv (Gamma ++ ((x, Uty tau_x)::nil)) ->
+    ~ appear_free_in_underty x tau ->
+    (forall e, tmR_in_ctx (Gamma ++ ((x, Uty tau_x)::nil)) tau e ->
+          (forall e_x, tmR_in_ctx Gamma tau_x e_x ->
+                  tmR_in_ctx Gamma tau (tlete x e_x e)
+          )
+    ).
+Proof with eauto.
+  intro Gamma.
+  induction Gamma; simpl; intros x tau_x tau Hinv Hfree e HeD e_x HexD.
+  - inversion Hinv; subst. apply app_eq_unit in H. destruct H; destruct H; subst.
+    + inversion H4; subst. apply H3 in HexD. repeat constructor... unfold under_tmR.
+      destruct H3 as (e_x & HexD & Hev). exists e_x. intros H
+
+                          
