proof/CtxInvariantSimp.v
@@ -1,0 +1,207 @@
+Set Warnings "-notation-overridden,-parsing".
+From PLF Require Import Maps.
+From PLF Require Import CoreLangSimp.
+From PLF Require Import NormalTypeSystemSimp.
+From PLF Require Import LinearContext.
+From PLF Require Import RfTypeDef.
+From PLF Require Import WellFormedSimp.
+From PLF Require Import DenotationSimp.
+From Coq Require Import Logic.FunctionalExtensionality.
+From Coq Require Import Logic.ClassicalFacts.
+From Coq Require Import Lists.List.
+
+Import CoreLangSimp.
+Import LinearContext.
+Import WellFormedSimp.
+Import DenotationSimp.
+Import ListNotations.
+
+(* It only makes sense when there is no duplicate bindings. *)
+Inductive ctx_inv: context -> Prop:=
+| ctx_inv_nil: ctx_inv nil
+| ctx_inv_cons_under: forall Gamma x (tau: overunderty),
+    well_formed_ctx (Gamma ++ ((x, tau)::nil)) ->
+    ctx_inv Gamma ->
+    l_find_right_most Gamma x = None ->
+    (forall e, tmR_in_ctx Gamma tau e -> (exists (v: value), e -->* v)) ->
+    ctx_inv (Gamma ++ ((x, tau)::nil)).
+
+Global Hint Constructors ctx_inv: core.
+
+(* reverse induction principle. *)
+Lemma ctx_inv_rev_inversion: forall Gamma x tau,
+    ctx_inv (Gamma ++ ((x, tau)::nil)) ->
+    (well_formed_ctx (Gamma ++ ((x, tau)::nil)) /\
+       ctx_inv Gamma /\
+       l_find_right_most Gamma x = None /\
+       (forall e, tmR_in_ctx Gamma tau e -> (exists (v: value), e -->* v))).
+Proof.
+  intros.
+  inversion H.
+  - apply app_one_eq_nil in H1. inversion H1.
+  - apply app_inj_tail in H0. destruct H0. inversion H5; subst. repeat split; auto.
+Qed.
+
+Lemma ctx_inv_implies_prefix_ctx_inv: forall Gamma2 Gamma1, ctx_inv (Gamma1 ++ Gamma2) -> ctx_inv Gamma1.
+Proof with eauto.
+  intro Gamma2.
+  induction Gamma2; intros Gamma1 H.
+  - rewrite app_nil_r in H...
+  - setoid_rewrite <- app_one_is_cons in H... rewrite app_assoc in H. apply IHGamma2 in H. inversion H...
+    + symmetry in H1. apply app_eq_nil in H1. destruct H1. inversion H1.
+    + apply app_inj_tail in H0. destruct H0; subst...
+Qed.
+
+Lemma ctx_inv_implies_well_formed: forall Gamma, ctx_inv Gamma -> well_formed_ctx Gamma.
+Proof with eauto.
+  apply (rev_ind (fun Gamma => ctx_inv Gamma -> well_formed_ctx Gamma))...
+  intros (x, xty) Gamma H Hconcat. inversion Hconcat. symmetry in H1. apply app_eq_nil in H1. destruct H1. inversion H1.
+  apply app_inj_tail in H0.
+  destruct H0; subst...
+Qed.
+
+Lemma ctx_inv_implies_fresh_binding_last:
+  forall Gamma x (tau_x: underty), ctx_inv (Gamma <l> x :l: Uty tau_x) -> ~ appear_free_in_underty x tau_x.
+Admitted.
+
+Lemma ctx_inv_implies_well_found_last:
+  forall Gamma x (tau_x: underty), ctx_inv (Gamma <l> x :l: Uty tau_x) -> well_formed Gamma tau_x.
+Admitted.
+
+Definition name_not_free_in_term {A: Type} (x: string) (e: tm): Prop.
+Admitted.
+
+Lemma ctx_inv_implies_postfix: forall a aty Gamma tau,
+  name_not_free_in_ctx_and_ty a Gamma tau ->
+  ctx_inv ((a, aty)::Gamma) ->
+  ctx_inv Gamma.
+Admitted.
+
+Lemma under_variable_has_same_type_in_ctx: forall Gamma x (tau: underty),
+    tmR_in_ctx (Gamma ++ ((x, Uty tau)::nil)) tau x.
+Admitted.
+
+Lemma over_variable_has_eq_type_in_ctx: forall Gamma x T phi,
+    tmR_in_ctx (Gamma ++ ((x, Oty ({{v: T | phi}}))::nil)) (mk_eq_var T x) x.
+Admitted.
+
+Lemma lete_ctx_inv_implies_safe_dropping_1_to_1: forall Gamma x tau_x tau,
+    ~ appear_free_in_underty x tau_x ->
+    ctx_inv (Gamma ++ ((x, Uty tau_x)::nil)) ->
+    (forall e, tmR_in_ctx (Gamma ++ ((x, Uty tau_x)::nil)) tau e ->
+          (forall e_x, tmR_in_ctx Gamma tau_x e_x -> tmR_in_ctx Gamma tau (tlete x e_x e))).
+Admitted.
+
+Lemma tletbiop_ctx_inv_implies_safe_dropping_1_to_1: forall Gamma x tau,
+    (forall e op (v1 v2: cid),
+        ctx_inv (Gamma ++ ((x, Uty (mk_op_retty_from_cids op v1 v2))::nil)) ->
+        tmR_in_ctx (Gamma ++ ((x, Uty (mk_op_retty_from_cids op v1 v2))::nil)) tau e ->
+        tmR_in_ctx (Gamma <l> x :l: ((mk_op_retty_from_cids op v1 v2))) tau e ->
+        tmR_in_ctx Gamma tau (tletbiop x op v1 v2 e)).
+Admitted.
+
+Lemma tletapp_oarr_ctx_inv_implies_safe_dropping_1_to_1: forall Gamma x tau_x tau,
+    (forall e (v1: value) (v2: cid) a T phi1,
+        tmR_in_ctx Gamma (a o: {{v: T | phi1}} o--> tau_x) v1 ->
+        tmR_in_ctx Gamma ([[v: T | phi1]]) v2 ->
+        ctx_inv (Gamma ++ ((x, Uty (under_subst_cid a v2 tau_x))::nil)) ->
+        tmR_in_ctx (Gamma ++ ((x, Uty (under_subst_cid a v2 tau_x))::nil)) tau e ->
+        tmR_in_ctx Gamma tau (tletapp x v1 v2 e)).
+Admitted.
+
+Lemma tletapp_arrarr_ctx_inv_implies_safe_dropping_1_to_1: forall Gamma x tau_x tau,
+    ~ appear_free_in_underty x tau_x ->
+    ctx_inv (Gamma ++ ((x, Uty tau_x)::nil)) ->
+    (forall e, tmR_in_ctx (Gamma ++ ((x, Uty tau_x)::nil)) tau e ->
+          (forall (v1 v2: value) t1,
+              tmR_in_ctx Gamma (t1 u--> tau_x) v1 ->
+              tmR_in_ctx Gamma t1 v2 ->
+              tmR_in_ctx Gamma tau (tletapp x v1 v2 e))).
+Admitted.
+
+
+(* Lemma ctx_inv_denotation_right_destruct: forall Gamma x (xty: underty) (tau: underty) e, *)
+(*     ctx_inv (Gamma ++ ((x, Uty xty)::nil)) -> *)
+(*     tmR_in_ctx (Gamma ++ ((x, Uty xty)::nil)) tau e -> *)
+(*     (name_not_free_in_ctx_and_ty x Gamma tau) -> *)
+(*     (exists e_x, tmR_in_ctx Gamma xty e_x /\ tmR_in_ctx Gamma tau (tlete x e_x e)). *)
+(* Proof with eauto. *)
+(*   intros Gamma. *)
+(*   induction Gamma; simpl; intros. *)
+(*   - inversion H0; subst. *)
+(*     + exfalso. apply H7... *)
+(*     + clear H7. destruct H8 as (e_x & HexD & HH). exists e_x. split... *)
+(*     + destruct H7 as (e_x & HexD & HH). exists e_x. split... *)
+(*     + destruct H7 as (e_x & HexD & HH). exists e_x. split... *)
+(*   - destruct a as (a, aty). destruct (eqb_spec a x). admit. (* a!= x*) destruct H1 as (Haty & H1). *)
+(*     inversion H0; subst. *)
+(*     + (* overtype *) admit. *)
+(*     + exfalso. admit. *)
+(*     + admit. *)
+(*     + destruct H7 as (e_a & Ha & HH). *)
+
+(*       destruct H8 as (e_x & Hex & HH). eapply free_ctx_inv_drop in H7... *)
+(*       eapply IHGamma in H7... destruct H7 as (e_a & Ha & HHH). *)
+(*       assert () *)
+(*       inversion H; subst. *)
+(*     destruct H1 as (Haty & HH). *)
+(*     destruct (eqb_spec x0 x). *)
+
+(*     destruct H7 as (e_x & HexD & HH). exists e_x. split... *)
+(*       constructor... constructor... inversion HH; subst. inversion H2; subst. *)
+(*       constructor... constructor...  *)
+
+Lemma tmR_in_ctx_pre_weakening: forall Gamma1 Gamma2 Gamma3 (tau: overunderty),
+    (Gamma1 ++ Gamma2) = Gamma3 ->
+    well_formed Gamma2 tau ->
+    (forall e, tmR_in_ctx Gamma2 tau e -> tmR_in_ctx Gamma3 tau e).
+Admitted.
+
+Lemma tmR_in_ctx_post_weakening: forall Gamma1 Gamma2 Gamma3 (tau: overunderty),
+    (Gamma1 ++ Gamma2) = Gamma3 ->
+    well_formed Gamma1 tau ->
+    (forall e, tmR_in_ctx Gamma1 tau e -> tmR_in_ctx Gamma3 tau e).
+Admitted.
+
+Lemma ctx_inv_drop_denoation: forall Gamma x xty,
+    ctx_inv ((x, xty)::Gamma) ->
+    (forall tau,
+        well_formed Gamma tau ->
+        (forall e, tmR_in_ctx Gamma tau e <-> tmR_in_ctx ((x, xty)::Gamma) tau e)).
+Proof with eauto.
+  intros Gamma.
+  induction Gamma; intros x xty H tau Hwf e; split; intros.
+  - eapply tmR_in_ctx_pre_weakening... rewrite app_nil_r...
+  - destruct xty. destruct u.
+    + inversion H0; subst.
+Admitted.
+
+
+(* Lemma tmR_in_ctx_post_weakening: forall Gamma (tau: underty), *)
+(*     well_formed l_empty tau -> *)
+(*     (forall e, tmR_in_ctx l_empty tau e -> tmR_in_ctx Gamma tau e). *)
+(* Proof with eauto. *)
+(* Admitted. *)
+
+
+(*       Lemma bigstep_lete: forall x e_x e (v: value), *)
+(*     ((tlete x e_x e) -->* v) <-> (exists (v_x: value), e_x -->* v_x /\ [x := v_x] e -->* v). *)
+(* Proof. *)
+(* Admitted. *)
+
+(* Lemma lete_preverse_denotation: forall tau x e_x e, *)
+(*     ~ (x \FVty tau) -> *)
+(*     under_tmR tau (tlete x e_x e) <-> *)
+(*       (exists (v_x: value), e_x -->* v_x -> under_tmR tau (subst x v_x e)). *)
+(* Proof with eauto. *)
+(*   intro tau. *)
+(*   induction tau; split; simpl; intros. *)
+(*   - inversion H. clear H. destruct H1 as (Hclose & HH). inversion H0; subst. *)
+(*     setoid_rewrite bigstep_lete in HH. *)
+(*     assert (empty |- v_x \Vin T1). eapply preservation_value... *)
+(*     split... eapply substitution_preserves_typing... *)
+(*     split... intros. apply bigstep_lete with (x:=x) (e:=e) (v:=c) in H0. *)
+(*     constructor. simpl. eapply substitution_preserves_typing... *)
+(*     constructor... simpl. eapply substitution_preserves_typing... *)
+(*     split... intros. *)
+(*     assert (tlete x v_x e -->* c)... inversion H6; subst. *)
